src/Common.v
@@ -1,4 +1,5 @@
 Require Export Coq.omega.Omega.
+Require Export Coq.Lists.List.
 Require Export bbv.Word.
 Require Export compiler.Monad.
 Require Export compiler.Decidable.
@@ -32,3 +33,14 @@ Instance Function_Map(K V: Type){decK: DecidableEq K}: Map (K -> option V) K V :
 Defined.
 
 Global Instance dec_eq_word : forall sz, DecidableEq (word sz) := weq.
+
+Lemma nth_error_nth: forall {T: Type} (l: list T) (e d: T) (i: nat),
+  nth_error l i = Some e ->
+  nth i l d = e.
+Proof.
+  intros T l. induction l; intros.
+  - destruct i; simpl in H; discriminate.
+  - destruct i; simpl in H; inversion H; subst.
+    + reflexivity.
+    + simpl. auto.
+Qed.
